<?xml version="1.0" encoding="UTF-8"?>
<rdf:RDF xmlns:bk="https://glossa.uni-graz.at/o:medea.bookkeeping" 
	xmlns:gams="https://gams.uni-graz.at/o:gams-ontology/#"
	xmlns:dc="http://purl.org/dc/elements/1.1/"
	xmlns:owl="http://www.w3.org/2002/07/owl#"
	xmlns:xsd="http://www.w3.org/2001/XMLSchema/rdf-schema" xmlns:rdf="http://www.w3.org/1999/02/22-rdf-syntax-ns#" xmlns:rdfs="http://www.w3.org/2000/01/rdf-schema#" xmlns:skos="http://www.w3.org/2004/02/skos/core#" xml:lang="en">
  <owl:Ontology rdf:about="https://glossa.uni-graz.at/o:medea.bookkeeping">
    <owl:versionInfo>Version 1.0</owl:versionInfo>
    <rdfs:label xml:lang="en">Bookkeeping Datamodel for Historical Accounts</rdfs:label>
    <rdfs:label xml:lang="de">Datenmodell für historische Rechnungsunterlagen</rdfs:label>
    <rdfs:comment xml:lang="en">This datamodel describes processes in historical accounting.</rdfs:comment>
    <rdfs:comment xml:lang="de">Dieses Datenmodell beschreibt Buchungsprozesse in historischen Rechnungsunterlagen</rdfs:comment>
    <rdfs:seeAlso rdf:resource="https://www.wikidata.org/wiki/Q4116214"></rdfs:seeAlso>
    <dc:description>This is a simple ontology for accounting facts: a transaction between two parties or accounts consists of at least one transfer from one to the other. It transfers a measurable
			and can be attested by text. The transfer occurs at a place and happens at a time. Booking a transfer into an account can create liabilities held by a party and owed to another.
			Measurables ar monetary values, commodities and prices. Services like work can also be transferd, but are not mandadory to be measurables. Prices can be considered as a special case of conversions of measurements. 
			A price is the quantity of payment or compensation given by one party to another in return for one unit of goods or services. The entry is an information fragment of a transfer often only naming one party as the other can be
			implicit in the textual context of the entry. A agent can act as deliverer of a measurable. When writing it down into the ledger, debit and credit are coded e.g. by using the appropriate columns in a table. Following the TEI model
			measurements have at least three properties: what is measured, what kind of unit is used, and in which quantity it is measured. In accounting theory an account can be &quot;personal&quot;, &quot;real&quot;,
			or &quot;nominal&quot;. It therefore can represent a relationship between two partners, an aggregation of items of value, or a temporary evaluation of the economic status of business. But accounts
			can also be considered as a list of bookkeeping entries. In accounting on paper they could be expressed in single pages or dedicated ledgers and they are identified by a heading. In final
			fair copies of bookkeeping documents in particular in the context of single entry bookkeeping they are just lists of entries. Fortunately there is a common abstraction in the two concepts
			when you consider accoun&quot; as method to organize a group of single facts. The account is an abstraction of personal account, real account and nominal account. </dc:description>
    <dc:title>Bookkeeping Datamodel for Historical Accounts</dc:title>
    <dc:creator>Christopher Pollin</dc:creator>
    <dc:creator>Georg Vogeler</dc:creator>
    <dc:date>2018</dc:date>
    <dc:identifier>https://glossa.uni-graz.at/o:medea.bookkeeping</dc:identifier>
    <dc:publisher>Zentrum für Informationsmodellierung, Universität Graz</dc:publisher>
    <dc:rights>https://creativecommons.org/licenses/by-nc-sa/4.0</dc:rights>
  </owl:Ontology>
  <rdfs:Class rdf:about="https://glossa.uni-graz.at/o:medea.bookkeeping#Transaction">
    <rdfs:label xml:lang="en">Transaction</rdfs:label>
    <rdfs:label xml:lang="de">Transaktion</rdfs:label>
    <rdfs:subClassOf rdf:resource="http://www.cidoc-crm.org/cidoc-crm/E28_Conceptual_Object"></rdfs:subClassOf>
    <rdfs:comment xml:lang="en">A financial transaction is an agreement, or communication, carried out between a buyer and a seller to exchange an asset for payment.</rdfs:comment>
    <rdfs:comment xml:lang="de">Transaktion ist in der Volkswirtschaftslehre die Übertragung von Wirtschaftsobjekten zwischen Wirtschaftssubjekten.</rdfs:comment>
    <rdfs:seeAlso rdf:resource="https://www.wikidata.org/wiki/Q1166072"></rdfs:seeAlso>
    <skos:example rdf:parseType="Literal">
    	<row ana="#bk_entry">
    		<cell><date ana="#bk_when" when="1828-09-22">22nd Septemper 1828</date></cell>
    		<cell>To order upon T. Smith for 3/</cell>
    		<cell>
    			<measure ana="#bk_money #bk_to" commodity="currency" quantity="50" unit="cents">50 cents</measure>
    		</cell>
    	</row>
    </skos:example>
  	<skos:example>
  		&lt;https://glossa.uni-graz.at/o:medea.wheaton.000#Entry-4-Transaction&gt; a &lt;bk:Transaction&gt;;
  		bk:consists-of &lt;https://glossa.uni-graz.at/o:medea.wheaton.000#Entry-4-Transfer-1&gt;;
  		bk:when "1828-09-22";
  		bk:entry "To order upon T. Smith for 3/ 50";  	
  		gams:isMemberOfCollection &lt;https://glossa.uni-graz.at/context:medea.wheaton&gt;.
  	</skos:example>
  </rdfs:Class>
  <rdfs:Class rdf:about="https://glossa.uni-graz.at/o:medea.bookkeeping#Transfer">
    <rdfs:label xml:lang="en">Transfer</rdfs:label>
    <rdfs:label xml:lang="de">Transfer</rdfs:label>
    <rdfs:subClassOf rdf:resource="http://www.cidoc-crm.org/cidoc-crm/E5_Event"></rdfs:subClassOf>
    <rdfs:comment xml:lang="en">A Transfer is the action in which one party cedes property rights to another parties or economic facts of an actor are assigned to an account.</rdfs:comment>
    <rdfs:comment xml:lang="de">Als Transfer versteht man die Aktion in der Geld, Waren o. Ä. von einem Konto oder Akteur zum anderen übermittelt wird.</rdfs:comment>
  	<skos:example>
  		&lt;https://glossa.uni-graz.at/o:medea.wheaton.000#Entry-10-Transfer-1&gt; a &lt;bk:Transfer&gt;;
  		bk:transfers &lt;https://glossa.uni-graz.at/o:medea.wheaton.000#Entry-10-Measurable-1&gt;;
  		bk:from &lt;https://glossa.uni-graz.at/o:medea.wheaton.000#Entry-10-pers_WCDH264&gt;;
  		bk:to &lt;https://glossa.uni-graz.at/o:medea.wheaton.000#Entry-10-#pers_MightyWheatonHimself&gt;.
  	</skos:example>
  </rdfs:Class>
  <rdfs:Class rdf:about="https://glossa.uni-graz.at/o:medea.bookkeeping#Between">
    <rdfs:label xml:lang="en">Between</rdfs:label>
    <rdfs:label xml:lang="de">Between</rdfs:label>
    <rdfs:subClassOf rdf:resource="http://www.cidoc-crm.org/cidoc-crm/E28_Conceptual_Object"></rdfs:subClassOf>
    <rdfs:comment xml:lang="en">A generic class for any concept which can be part of transaction in abstract bookkeeping, which connects bk_from and bk_to.</rdfs:comment>
    <rdfs:comment xml:lang="de">Ein genersiche Klasse, das bk_from und bk_to in Verbindung setzt.</rdfs:comment>
  	<skos:example>
  		&lt;https://glossa.uni-graz.at/o:medea.wheaton.000#Entry-1-pers_WCDH524&gt; a &lt;bk:Between&gt;;
  			bk:name "Pliny Puffer".
  	</skos:example>
  </rdfs:Class>
  <rdfs:Class rdf:about="https://glossa.uni-graz.at/o:medea.bookkeeping#Agent">
    <rdfs:subClassOf rdf:resource="http://www.cidoc-crm.org/cidoc-crm/E39_Actor"></rdfs:subClassOf>
    <rdfs:label xml:lang="en">Agent</rdfs:label>
    <rdfs:label xml:lang="de">Vermittler</rdfs:label>
    <rdfs:comment xml:lang="en">Someone delivers something for somebody.</rdfs:comment>
    <rdfs:comment xml:lang="de"></rdfs:comment>
    <skos:example rdf:parseType="Literal">
			100 $ to 
		</skos:example>
  </rdfs:Class>
  <rdfs:Class rdf:about="https://glossa.uni-graz.at/o:medea.bookkeeping#TypeAssignment">
    <rdfs:subClassOf rdf:resource="http://www.cidoc-crm.org/cidoc-crm/E17_Type_Assignment"></rdfs:subClassOf>
    <rdfs:label xml:lang="en">Type Assignment</rdfs:label>
    <rdfs:label xml:lang="de">Typenzuordnung</rdfs:label>
    <rdfs:comment xml:lang="en">Comprises the actions of classifying items of whatever kind. Such items include objects, specimens, people, actions and concepts. This classification (interpretation) is done by the scholar.</rdfs:comment>
    <rdfs:comment xml:lang="de">Fasst Transaktionen als fachwissenschaftliche Interpretation zusammen.</rdfs:comment>
    <skos:example rdf:parseType="Literal">
      <div ana="#bk_entry">
        ToDo
      </div>
    </skos:example>
    <skos:example>
      &lt;bk:Transaction&gt; bk:typeAssignment &lt;https://glossa.uni-graz.at/o:medea.wheaton.000#Entry-1-Project_1&gt;.
    </skos:example>
    <skos:example>
      &lt;bk:Transaction&gt; bk:typeAssignment &lt;https://glossa.uni-graz.at/o:medea.wheaton.000#Entry-1-Context_1&gt;.
    </skos:example>
  </rdfs:Class>
  <rdfs:Class rdf:about="https://glossa.uni-graz.at/o:medea.bookkeeping#Account">
    <rdfs:label xml:lang="en">Account</rdfs:label>
    <rdfs:label xml:lang="de">Konto</rdfs:label>
    <rdfs:subClassOf rdf:resource="https://glossa.uni-graz.at/o:medea.bookkeeping#Between"></rdfs:subClassOf>
    <rdfs:comment xml:lang="en">An account refers to assets, liabilities, income, expenses, and equity, as represented by individual ledger pages, to which changes in value are chronologically
			recorded with debit and credit entries. These entries, referred to as postings, become part of a book of final entry or ledger. </rdfs:comment>
    <rdfs:comment xml:lang="de">Ein Konto ist die zentrale Datenstruktur in der Buchführung sowie im Zahlungsverkehr.</rdfs:comment>
    <rdfs:seeAlso rdf:resource="https://www.wikidata.org/wiki/Q508295"></rdfs:seeAlso>
    <skos:example rdf:parseType="Literal">
      <span ana="#bk_from #bk_Account" ref="#acc_1">Cash Account</span>
    </skos:example>
  	<skos:example>
  		&lt;https://glossa.uni-graz.at/o:medea.wheaton.000#Entry-1-acc_1&gt; a &lt;bk:Account&gt;;
  		bk:name "Cash Account".
  	</skos:example>
  </rdfs:Class>
  <rdfs:Class rdf:about="https://glossa.uni-graz.at/o:medea.bookkeeping#Party">
    <rdfs:label xml:lang="en">Party</rdfs:label>
    <rdfs:label xml:lang="de">Akteur</rdfs:label>
    <rdfs:subClassOf rdf:resource="https://glossa.uni-graz.at/o:medea.bookkeeping#Between"></rdfs:subClassOf>
    <rdfs:subClassOf rdf:resource="http://www.cidoc-crm.org/cidoc-crm/E39_Actor"></rdfs:subClassOf>
    <rdfs:comment xml:lang="en">An actor in a transaction.</rdfs:comment>
    <rdfs:comment xml:lang="de">Ein Akteur in einer Transaktion.</rdfs:comment>
    <rdfs:seeAlso rdf:resource="https://www.wikidata.org/wiki/Q508295"></rdfs:seeAlso>
    <skos:example rdf:parseType="Literal">
      <name ana="#bk_from #bk_Party" ref="#person_1">Christopher</name>
    </skos:example>
  </rdfs:Class>
  <rdfs:Class rdf:about="https://glossa.uni-graz.at/o:medea.bookkeeping#Measurable">
    <rdfs:label xml:lang="en">Measurable</rdfs:label>
    <rdfs:label xml:lang="de">Quantifizierbares</rdfs:label>
    <rdfs:subClassOf rdf:resource="http://www.cidoc-crm.org/cidoc-crm/E71_Man-Made_Thing"></rdfs:subClassOf>
    <rdfs:comment xml:lang="en">Everything that is countable.</rdfs:comment>
    <rdfs:comment xml:lang="de">Alles was quantifiziert (gezählt) werden kann</rdfs:comment>
  </rdfs:Class>
  <rdfs:Class rdf:about="https://glossa.uni-graz.at/o:medea.bookkeeping#Commodity">
    <rdfs:label xml:lang="en">Commodity</rdfs:label>
    <rdfs:label xml:lang="de">Ware</rdfs:label>
    <rdfs:subClassOf rdf:resource="https://glossa.uni-graz.at/o:medea.bookkeeping#Measurable"></rdfs:subClassOf>
    <rdfs:comment xml:lang="en">A commodity is an economic good</rdfs:comment>
    <rdfs:comment xml:lang="de">Handelsware ist eine Sammelbezeichnung für die von Gewerbetreibenden umgesetzten materiellen Wirtschaftsgüter.</rdfs:comment>
    <rdfs:seeAlso rdf:resource="https://www.wikidata.org/wiki/Q317088"></rdfs:seeAlso>
    <skos:example rdf:parseType="Literal">
      <div ana="#bk_entry">
        <measure ana="#bk_commodity" commodity="commodity" quantity="1" unit="cow">1 cow</measure>
      </div>
    </skos:example>
    <skos:example rdf:parseType="Literal">
      <measure ana="#bk_commodity" commodity="sugar" quantity="1" unit="lb">1 lb Sugar</measure>
    </skos:example>
    <skos:example> bk_when;bk_text;bk_from;bk_to;bk_commodity 1690-10-01;Christopher gives Georg 1 cow ;Christopher;Georg;1 cow </skos:example>
    <skos:example> bk_when;bk_text;bk_from;bk_to;bk_money;bk_commodity 1690-10-01;Christopher buys 3 bags rice from Georg for 10 €;Christopher;Georg;10 (€);3 (bags rice) </skos:example>
  </rdfs:Class>
  <rdfs:Class rdf:about="https://glossa.uni-graz.at/o:medea.bookkeeping#Service">
    <rdfs:label xml:lang="en">Service</rdfs:label>
    <rdfs:label xml:lang="de">Dienstleistung</rdfs:label>
    <rdfs:subClassOf rdf:resource="http://www.cidoc-crm.org/cidoc-crm/E5_Event"></rdfs:subClassOf>
    <rdfs:subClassOf rdf:resource="https://glossa.uni-graz.at/o:medea.bookkeeping#Measurable"></rdfs:subClassOf>
    <rdfs:comment xml:lang="en">A service is a transaction in which no physical goods are transferred from the seller to the buyer.</rdfs:comment>
    <rdfs:comment xml:lang="de">Ein immaterielles Gut, das entsteht, wenn ein Wirtschaftssubjekt für ein anderes eine entgeltliche Tätigkeit ausübt</rdfs:comment>
    <rdfs:seeAlso rdf:resource="https://www.wikidata.org/wiki/Q7406919"></rdfs:seeAlso>
    <skos:example rdf:parseType="Literal">
      <measure ana="#bk_service" commodity="work" quantity="3" unit="hours"> cutting trees for 3 hours.</measure>
    </skos:example>
    <skos:example rdf:parseType="Literal">
      <span ana="#bk_service">By work</span>
    </skos:example>
    <skos:example> bk_whe;bk_text;bk_from;bk_to;bk_money;bk_commodity; 2018-10-01;Christopher buys 3 bags rice from Georg for 10 €;Christopher;Georg;10 (€);3 (bags rice) </skos:example>
  </rdfs:Class>
  <rdfs:Class rdf:about="https://glossa.uni-graz.at/o:medea.bookkeeping#MonetaryValue">
    <rdfs:label xml:lang="en">Monetary Value</rdfs:label>
    <rdfs:label xml:lang="de">Geldwert</rdfs:label>
    <rdfs:subClassOf rdf:resource="https://glossa.uni-graz.at/o:medea.bookkeeping#Measurable"></rdfs:subClassOf>
    <rdfs:comment xml:lang="en">The amount of value an item or a service has in relation to if it were sold for cash to a willing buyer. A Monetary Value can consist of subtotals, which are monetary values too. </rdfs:comment>
    <rdfs:comment xml:lang="de">Geldwert ist in der Volkswirtschaftslehre das Austauschverhältnis zwischen Geld und Gütern oder Dienstleistungen.</rdfs:comment>
    <rdfs:seeAlso rdf:resource="https://www.wikidata.org/wiki/Q1499548"></rdfs:seeAlso>
    <skos:example rdf:parseType="Literal">
      <measure ana="#bk_money" commodity="currency" quantity="1" unit="dollars">1 $</measure>
      <measure ana="#bk_money" commodity="currency" quantity="50" unit="gams.uni-graz.at/currency#cents">50 c</measure>
    </skos:example>
    <skos:example> bk_when;bk_text;bk_from;bk_to;bk_money; 1808-08-01;1/4 lb Powder 2/6 2 lb Shot 5/;Stagville;William Pettigrew Jr.;7 (s) 6 (d);0,25 (lb Powder) 0.33 (lb Shot) </skos:example>
  </rdfs:Class>
  <rdfs:Class rdf:about="https://glossa.uni-graz.at/o:medea.bookkeeping#Price">
    <rdfs:label xml:lang="en">Price</rdfs:label>
    <rdfs:label xml:lang="de">Preis</rdfs:label>
    <rdfs:subClassOf rdf:resource="https://glossa.uni-graz.at/o:medea.bookkeeping#Measurable"></rdfs:subClassOf>
    <rdfs:comment xml:lang="en">The quantity of payment or compensation given by one party to another in return for one unit of goods or services.</rdfs:comment>
    <rdfs:comment xml:lang="de">In Geldeinheiten gezahlte Gegenleistung für eine bestimmte Mengeneinheit von erworbenen Produkten oder Dienstleistungen</rdfs:comment>
    <rdfs:seeAlso rdf:resource="https://www.wikidata.org/wiki/Q160151"></rdfs:seeAlso>
    <skos:example rdf:parseType="Literal">
      <measure ana="#bk_commodity" commodity="powder" quantity="0.25" unit="lb">1/4 lb Powder 
				<measure ana="#bk_price" commodity="currency" quantity="2" unit="s">2</measure>/<measure ana="#bk_price" commodity="currency" quantity="6" unit="d">6</measure>
      </measure>
      <measure ana="#bk_commodity" commodity="sugar" quantity="1" unit="lb">1 lb Sugar <measure ana="#bk_price" commodity="currency" quantity="3" unit="s">3</measure>/<measure ana="#bk_price" commodity="currency" quantity="4" unit="d">4</measure>
      </measure>
    </skos:example>
    <skos:example> 
			bk_when;bk_text;bk_from;bk_to;bk_money;bk_commodity;bk_price 2018-10-01;Georg buys a hundred bags rice from Christopher for 6 € for each bag;Georg;Christopher;600 (€);100 (bags
			rice);6 (€)
		</skos:example>
  </rdfs:Class>
  <rdf:Property rdf:about="https://glossa.uni-graz.at/o:medea.bookkeeping#transfers">
    <rdfs:label xml:lang="en">transfer</rdfs:label>
    <rdfs:label xml:lang="de">übermitteln</rdfs:label>
    <rdfs:comment xml:lang="en">A transfer conveys something.</rdfs:comment>
    <rdfs:comment xml:lang="de">Etwas wird an jemand anderen übermittel</rdfs:comment>
    <rdfs:domain rdf:resource="https://glossa.uni-graz.at/o:medea.bookkeeping#Transfer"></rdfs:domain>
    <rdfs:range rdf:resource="https://glossa.uni-graz.at/o:medea.bookkeeping#Measurable"></rdfs:range>
  </rdf:Property>
  <rdf:Property rdf:about="https://glossa.uni-graz.at/o:medea.bookkeeping#from">
    <rdfs:label xml:lang="en">from</rdfs:label>
    <rdfs:label xml:lang="de">von</rdfs:label>
    <rdfs:comment xml:lang="en">Something goes away from somebody. An account decreases.</rdfs:comment>
    <rdfs:comment xml:lang="de">Etwas geht von einem Akteur / Konto weg.</rdfs:comment>
    <rdfs:domain rdf:resource="https://glossa.uni-graz.at/o:medea.bookkeeping#Transfer"></rdfs:domain>
    <rdfs:range rdf:resource="https://glossa.uni-graz.at/o:medea.bookkeeping#Between"></rdfs:range>
    <skos:example rdf:parseType="Literal"></skos:example>
  </rdf:Property>
  <rdf:Property rdf:about="https://glossa.uni-graz.at/o:medea.bookkeeping#to">
    <rdfs:label xml:lang="en">to</rdfs:label>
    <rdfs:label xml:lang="de">nach</rdfs:label>
    <rdfs:comment xml:lang="en">Something goes to somebody. An account increases.</rdfs:comment>
    <rdfs:comment xml:lang="de">Etwas geht zu einem Akteur / Konto.</rdfs:comment>
    <rdfs:domain rdf:resource="https://glossa.uni-graz.at/o:medea.bookkeeping#Transfer"></rdfs:domain>
    <rdfs:range rdf:resource="https://glossa.uni-graz.at/o:medea.bookkeeping#Between"></rdfs:range>
    <skos:example rdf:parseType="Literal">
      <div>
        <head ana="#bk_to" ref="bs_StadtWeinungeld-div-0">Weinungeld</head>
        <p ana="#bk_entry" xml:id="bs_Zahlungen-1"> Prima angaria <measure quantity="1804" type="currency" unit="https://glossa.uni-graz.at#lb"> xviij <seg rend="super">c</seg> iiij lb </measure>
          <measure quantity="4" type="currency" unit="ß-w">iiij ß</measure>
          <measure quantity="10" type="currency" unit="d">x d</measure>
        </p>
        <p ana="#bk_entry" xml:id="bs_Zahlungen-2"> Secunda angaria <measure quantity="1797" type="currency" unit="lb"> j <seg rend="super">m</seg> vij <seg rend="super">c</seg> lxxxxvij lb </measure>
          <measure quantity="16" type="currency" unit="ß-w">xvj ß</measure>
          <measure quantity="1" type="currency" unit="d">j d</measure>
        </p>
      </div>
    </skos:example>
    <skos:example rdf:parseType="Literal">
      <span ana="#bk_entry">
        <orgName ana="#bk_to #bk_account" ref="#Acc.1">Christophers Account</orgName> receives on the <date ana="#bk_when" when="1460-10-01">10.01.1460</date>
      </span>
    </skos:example>
  </rdf:Property>
  <rdf:Property rdf:about="https://glossa.uni-graz.at/o:medea.bookkeeping#consistsOf">
    <rdfs:label xml:lang="en">consists of</rdfs:label>
    <rdfs:label xml:lang="de">besteht aus</rdfs:label>
    <rdfs:comment xml:lang="en">A transaction consists of a number of transfers</rdfs:comment>
    <rdfs:comment xml:lang="de">Eine Transaktion besteht aus mehreren Transfers.</rdfs:comment>
    <rdfs:domain rdf:resource="https://glossa.uni-graz.at/o:medea.bookkeeping#Transaction"></rdfs:domain>
    <rdfs:range rdf:resource="https://glossa.uni-graz.at/o:medea.bookkeeping#Transfer"></rdfs:range>
    
  </rdf:Property>
  <rdf:Property rdf:about="https://glossa.uni-graz.at/o:medea.bookkeeping#entry">
    <rdfs:label xml:lang="en">entry</rdfs:label>
    <rdfs:label xml:lang="de">hat Eintrag</rdfs:label>
    <rdfs:comment xml:lang="en">A transfer has a physical representation (text) in a source.</rdfs:comment>
    <rdfs:comment xml:lang="de">Ein Transfer besitz einen physische (textuelle) Representation in einer Quelle.</rdfs:comment>
  	<rdfs:domain rdf:resource="https://glossa.uni-graz.at/o:medea.bookkeeping#Transaction"></rdfs:domain>
  	<rdfs:range rdf:resource="http://www.w3.org/2000/01/rdf-schema#Literal"></rdfs:range>
  	<skos:example rdf:parseType="Literal">
  		<div ana="bk_entry">To ax dlvd By Puffer 9/1</div>
  	</skos:example>
  	<skos:example>&lt;bk:Transaction&gt; bk:entry "To ax dlvd By Puffer 9/1 1 50".</skos:example>
  </rdf:Property>
  <rdf:Property rdf:about="https://glossa.uni-graz.at/o:medea.bookkeeping#assignment">
    <rdfs:label xml:lang="en">assigned</rdfs:label>
    <rdfs:label xml:lang="de">zugeordnet</rdfs:label>
    <rdfs:comment xml:lang="en">Assigns transactions to a specific type or context. This decision is made by a scholar and is an interpretation.</rdfs:comment>
    <rdfs:comment xml:lang="de">Ordnet Transaktionen einem bestimmten Typ bzw. Kontext zu. Diese Entscheidung wird vom Fachwissenschaftler getroffen und ist eine Interpretation.</rdfs:comment>
    <rdfs:domain rdf:resource="https://glossa.uni-graz.at/o:medea.bookkeeping#Transaction"></rdfs:domain>
    <rdfs:range rdf:resource="https://glossa.uni-graz.at/o:medea.bookkeeping#TypeAssignment"></rdfs:range>
    <rdfs:subPropertyOf rdf:resource="http://www.cidoc-crm.org/cidoc-crm/P42_assigned"></rdfs:subPropertyOf>
    <skos:example rdf:parseType="Literal">
      ToDo
    </skos:example>
    <skos:example>ToDo</skos:example>
  </rdf:Property>
  <rdf:Property rdf:about="https://glossa.uni-graz.at/o:medea.bookkeeping#by">
    <rdfs:label xml:lang="en">by</rdfs:label>
    <rdfs:label xml:lang="de">bei</rdfs:label>
    <rdfs:comment xml:lang="en">A transfer can be deliverd by an bk:Agent</rdfs:comment>
    <rdfs:comment xml:lang="de">Ein Transfer kann durch eine dritte Person vermittelt werden.</rdfs:comment>
    <rdfs:domain rdf:resource="https://glossa.uni-graz.at/o:medea.bookkeeping#Transfer"></rdfs:domain>
    <rdfs:range rdf:resource="https://glossa.uni-graz.at/o:medea.bookkeeping#Agent"></rdfs:range>
  	<skos:example rdf:parseType="Literal">
  		To ax dlvd <name ana="#bk_by" ref="pers.1">By Puffer</name> 9/1 
  	</skos:example>
  	<skos:example>&lt;bk:Transfer&gt; bk:by &lt;https://glossa.uni-graz.at/o:medea.wheaton.000#Entry-0-pers.1&gt;.</skos:example>
  </rdf:Property>
  <rdf:Property rdf:about="https://glossa.uni-graz.at/o:medea.bookkeeping#price">
    <rdfs:label xml:lang="en">price</rdfs:label>
    <rdfs:label xml:lang="de">hat Preis</rdfs:label>
  	<rdfs:comment xml:lang="en">A bk:Commodity or a bk:Service have a bk:Price.</rdfs:comment>
    <rdfs:comment xml:lang="de">Etwas hat einen Preis.</rdfs:comment>
    <rdfs:domain rdf:resource="https://glossa.uni-graz.at/o:medea.bookkeeping#Commodity"></rdfs:domain>
    <rdfs:domain rdf:resource="https://glossa.uni-graz.at/o:medea.bookkeeping#Service"></rdfs:domain>
    <rdfs:range rdf:resource="https://glossa.uni-graz.at/o:medea.bookkeeping#Price"></rdfs:range>
  	<skos:example rdf:parseType="Literal">
  		<measure ana="#bk_price" commodity="currency" quantity="5" unit="dollar">5 $</measure>
  	</skos:example>
  	<skos:example>&lt;bk:Commodity&gt; bk:price &lt;bk:Price&gt;.</skos:example>
  </rdf:Property>
  <rdf:Property rdf:about="https://glossa.uni-graz.at/o:medea.bookkeeping#text">
    <rdfs:label xml:lang="en">text</rdfs:label>
    <rdfs:label xml:lang="de">Textknoten</rdfs:label>
    <rdfs:comment xml:lang="en">the textual representation of an entitiy.</rdfs:comment>
    <rdfs:comment xml:lang="de">Eine textuelle Referenz einer Entität</rdfs:comment>
    <rdfs:domain rdf:resource="https://glossa.uni-graz.at/o:medea.bookkeeping#Measurable"></rdfs:domain>
  	<rdfs:range rdf:resource="http://www.w3.org/2000/01/rdf-schema#Literal"></rdfs:range>
    <skos:example rdf:parseType="Literal">
      <measure ana="#bk_service">5 hours of work</measure>
    </skos:example>
  	<skos:example>&lt;Service&gt; bk:text "5 hours of work".</skos:example>
  </rdf:Property>
  <rdf:Property rdf:about="https://glossa.uni-graz.at/o:medea.bookkeeping#debit">
    <rdfs:label xml:lang="en">debit</rdfs:label>
    <rdfs:label xml:lang="de">Soll</rdfs:label>
  	<rdfs:comment xml:lang="en">Marks an bk:Transfer as a Transfer to a credit account. The money obtained with the credits is destined as debit in transaction accountsm like assets.</rdfs:comment>
  	<rdfs:comment xml:lang="de">Markiert eine bk:Transfer als einen Transfer auf ein ein Soll-Konto, wie z.B. Vermögenswerte wie Bar- und Bankvermögen.</rdfs:comment>
    <rdfs:domain rdf:resource="https://glossa.uni-graz.at/o:medea.bookkeeping#Transfer"></rdfs:domain>
    <rdfs:range rdf:resource="http://www.w3.org/2001/XMLSchema#boolean"></rdfs:range>
    <rdfs:seeAlso rdf:resource="https://www.wikidata.org/wiki/Q5248104"></rdfs:seeAlso>
  	<skos:example rdf:parseType="Literal">
  		<name ana="#bk_to #bk_debit" ref="#debitAccount.1">Cash Account</name>
  	</skos:example>
  	<skos:example>&lt;bk:Transfer&gt; bk:debit "true".</skos:example>
  	<skos:example>&lt;bk:Transfer&gt; bk:debit "false".</skos:example>
  </rdf:Property>
  <rdf:Property rdf:about="https://glossa.uni-graz.at/o:medea.bookkeeping#credit">
    <rdfs:label xml:lang="en">credit</rdfs:label>
    <rdfs:label xml:lang="de">Haben</rdfs:label>
    <rdfs:comment xml:lang="en">Marks an bk:Transfer as a Transfer to a credit account. The sources for spending money in transaction account is credit, like liabilities</rdfs:comment>
  	<rdfs:comment xml:lang="de">Markiert eine bk:Transfer als einen Transfer auf ein ein Haben-Konto, wie z.B. Verbindlichkeiten wie Kredite und Schulden.</rdfs:comment>
    <rdfs:domain rdf:resource="https://glossa.uni-graz.at/o:medea.bookkeeping#Transfer"></rdfs:domain>
    <rdfs:range rdf:resource="http://www.w3.org/2001/XMLSchema#boolean"></rdfs:range>
    <rdfs:seeAlso rdf:resource="https://www.wikidata.org/wiki/Q305253"></rdfs:seeAlso>
  	<skos:example rdf:parseType="Literal">
  		<name ana="#bk_to #bk_credit" ref="11833">Credit Account</name>
  	</skos:example>
  	<skos:example>&lt;bk:Transfer&gt; bk:credit "true".</skos:example>
  	<skos:example>&lt;bk:Transfer&gt; bk:credit "false".</skos:example>
  </rdf:Property>
	<rdf:Property rdf:about="https://glossa.uni-graz.at/o:medea.bookkeeping#commodity">
		<rdfs:label xml:lang="en">commodity</rdfs:label>
		<rdfs:label xml:lang="de">hat Anzahl</rdfs:label>
		<rdfs:comment xml:lang="en">A bk:Commodity or bk:Service can be classified."</rdfs:comment>
		<rdfs:comment xml:lang="de">Ein bk:Commodity oder bk:Service wird klassifiziert.</rdfs:comment>
		<rdfs:domain rdf:resource="https://glossa.uni-graz.at/o:medea.bookkeeping#Commodity"/>
		<rdfs:domain rdf:resource="https://glossa.uni-graz.at/o:medea.bookkeeping#Service"/>
		<rdfs:range rdf:resource="http://www.w3.org/2000/01/rdf-schema#Literal"></rdfs:range>
		<rdfs:range rdf:resource="http://www.w3.org/2001/XMLSchema/rdf-schema#anyURI"/>
		<skos:example rdf:parseType="Literal">
			<measure ana="#bk_commodity" commodity="wood" quantity="10" unit="sticks">10 wooden sticks</measure>
		</skos:example>
		<skos:example rdf:parseType="Literal">
			<measure ana="#bk_service" commodity="cutting" quantity="2" unit="h">cutting sticks for two hours</measure>
		</skos:example>
		<skos:example>&lt;bk:Commodity&gt; bk:unit "bushels"; bk:quantity "2"; bk:commodity "potatoes".</skos:example>
	</rdf:Property>
  <rdf:Property rdf:about="https://glossa.uni-graz.at/o:medea.bookkeeping#quantity">
    <rdfs:label xml:lang="en">quantity</rdfs:label>
    <rdfs:label xml:lang="de">hat Anzahl</rdfs:label>
    <rdfs:comment xml:lang="en">A measurable can be counted and has a decimal value.</rdfs:comment>
    <rdfs:comment xml:lang="de"></rdfs:comment>
    <rdfs:domain rdf:resource="https://glossa.uni-graz.at/o:medea.bookkeeping#Measurable"></rdfs:domain>
    <rdfs:range rdf:resource="http://www.w3.org/2001/XMLSchema#decimal"></rdfs:range>
  	<skos:example rdf:parseType="Literal">
      <measure ana="#bk_money" commodity="currency" quantity="20" unit="dollar">20 $</measure>
    </skos:example>
  	<skos:example>&lt;bk:Money&gt; bk:unit "dollars"; bk:quantity "30"; bk:text "thirty dollars".</skos:example>
  </rdf:Property>
	<rdf:Property rdf:about="https://glossa.uni-graz.at/o:medea.bookkeeping#unit">
    <rdfs:label xml:lang="en">unit</rdfs:label>
    <rdfs:label xml:lang="de">hat Einheit</rdfs:label>
    <rdfs:comment xml:lang="en">A Measurable has a unit. Can be a string or a URI or encoded in the TEI.</rdfs:comment>
    <rdfs:comment xml:lang="de"></rdfs:comment>
    <rdfs:domain rdf:resource="https://glossa.uni-graz.at/o:medea.bookkeeping#Measurable"></rdfs:domain>
    <rdfs:range rdf:resource="http://www.w3.org/2000/01/rdf-schema#Literal"></rdfs:range>
  	<rdfs:range rdf:resource="http://www.w3.org/2001/XMLSchema/rdf-schema#anyURI"/>
  	<skos:example rdf:parseType="Literal">
      <measure ana="#bk_service" commodity="time" quantity="5" unit="hours">5 hours of work</measure>
  	</skos:example>
  	<skos:example rdf:parseType="Literal">
      <measure ana="#bk_money" commodity="currency" quantity="20" unit="dollar">20 $</measure>
    </skos:example>
  	<skos:example>
  		&lt;bk:Money&gt; bk:unit "dollar".
  	</skos:example>
  	<skos:example>
  		&lt;bk:Commodity&gt; bk:unit &lt;https://www.wikidata.org/wiki/Q11570&gt;.
  	</skos:example>
  </rdf:Property>
	<rdf:Property rdf:about="https://glossa.uni-graz.at/o:medea.bookkeeping#when">
		<rdfs:label xml:lang="en">when</rdfs:label>
		<rdfs:label xml:lang="de">hat Zeitraum</rdfs:label>
		<rdfs:comment xml:lang="en">A bk:Transfer can be related to a date.</rdfs:comment>
		<rdfs:comment xml:lang="de">Stellt die Verbindung zu einer Zeitangabe her.</rdfs:comment>
		<rdfs:domain rdf:resource="https://glossa.uni-graz.at/o:medea.bookkeeping#Transaction"></rdfs:domain>
		<rdfs:range rdf:resource="http://www.w3.org/2001/XMLSchema#dateTime"></rdfs:range>
		<skos:example rdf:parseType="Literal">
			<date ana="#bk_when" when="1750-06-10">10. July 1750</date>
		</skos:example>
		<skos:example>
			&lt;bk:Transaction&gt; bk:when "1750-06-10".
		</skos:example>
	</rdf:Property>
	<rdf:Property rdf:about="https://glossa.uni-graz.at/o:medea.bookkeeping#where">
		<rdfs:label xml:lang="en">where</rdfs:label>
		<rdfs:label xml:lang="de">hat Ort</rdfs:label>
		<rdfs:comment xml:lang="en">A Transaction can be related to a place. Define as a literal like &quot;Graz&quot; or more specific by a reference</rdfs:comment>
		<rdfs:comment xml:lang="de">Eine Transaction steht mit einem Ort in Verbindung</rdfs:comment>
		<rdfs:domain rdf:resource="https://glossa.uni-graz.at/o:medea.bookkeeping#Transaction"></rdfs:domain>
		<rdfs:range rdf:resource="http://www.w3.org/2000/01/rdf-schema#Literal"/>
		<rdfs:range rdf:resource="http://www.w3.org/2001/XMLSchema/rdf-schema#anyURI"/>
		<skos:example rdf:parseType="Literal">
			<placeName ana="#bk_where" ref="http://www.geonames.org/2778067">Graz</placeName>
		</skos:example>
		<skos:example>
			&lt;bk:Transaction&gt; bk:where "Graz".
		</skos:example>
		<skos:example>
			&lt;bk:Transaction&gt; bk:where &lt;http://www.geonames.org/2778067&gt;.
		</skos:example>
	</rdf:Property>	
  <rdf:Property rdf:about="https://glossa.uni-graz.at/o:medea.bookkeeping#name">
    <rdfs:label xml:lang="en">name</rdfs:label>
    <rdfs:label xml:lang="de">genannt</rdfs:label>
    <rdfs:comment xml:lang="en">Gives a Party or an Account a name.</rdfs:comment>
    <rdfs:comment xml:lang="de">Text der im bk_Entry steht. Für Volltextsuche verwendet</rdfs:comment>
    <rdfs:domain rdf:resource="https://glossa.uni-graz.at/o:medea.bookkeeping#Account"></rdfs:domain>
    <rdfs:domain rdf:resource="https://glossa.uni-graz.at/o:medea.bookkeeping#Party"></rdfs:domain>
    <rdfs:range rdf:resource="http://www.w3.org/2000/01/rdf-schema#Literal"></rdfs:range>
  	<skos:example  rdf:parseType="Literal">
  		<name ana="#bk_to" ref="LMWcash" type="account">cash</name>
  	</skos:example>
  	<skos:example>
  		&lt;bk:Account&gt; bk:name "Cash Account".
  	</skos:example>
  	<skos:example>
  		&lt;bk:Party&gt; bk:name "Darius Drake".
  	</skos:example>
  </rdf:Property>
  <rdf:Property rdf:about="https://glossa.uni-graz.at/o:medea.bookkeeping#commentary">
    <rdfs:label xml:lang="en">name</rdfs:label>
    <rdfs:label xml:lang="de">genannt</rdfs:label>
    <rdfs:comment xml:lang="en">Gives a Party or an Account a name.</rdfs:comment>
    <rdfs:comment xml:lang="de">Text der im bk_Entry steht. Für Volltextsuche verwendet</rdfs:comment>
    <rdfs:domain rdf:resource="https://glossa.uni-graz.at/o:medea.bookkeeping#TypeAssignment"></rdfs:domain>
    <rdfs:range rdf:resource="http://www.w3.org/2000/01/rdf-schema#Literal"></rdfs:range>
    <skos:example  rdf:parseType="Literal">
      ToDo
    </skos:example>
    <skos:example>
      &lt;https://glossa.uni-graz.at/o:medea.wheaton.000#Entry-1-Project_1&gt; bk:commentary "Schlitz Companys investments from 1911 to 1913" .
    </skos:example>
    <skos:example>
      &lt;bk:Transaction&gt; bk:commentary "All transactions in connection with slavetrade at Washingtons farm X".
    </skos:example>
  </rdf:Property>
  <rdf:Property rdf:about="https://glossa.uni-graz.at/o:medea.bookkeeping#status">
    <rdfs:label xml:lang="en">transaction status</rdfs:label>
    <rdfs:label xml:lang="de">hat Status</rdfs:label>
    <rdfs:comment xml:lang="en">Specifies the status of a transaction.</rdfs:comment>
    <rdfs:comment xml:lang="de">Spezifiziert den Status einer Transaktion weiter.</rdfs:comment>
    <rdfs:domain rdf:resource="https://glossa.uni-graz.at/o:medea.bookkeeping#Transaction"></rdfs:domain>
    <rdfs:range rdf:resource="http://www.w3.org/2000/01/rdf-schema#Literal"></rdfs:range>
    <skos:example  rdf:parseType="Literal">
      ToDo
    </skos:example>
    <skos:example>
      &lt;bk:Transaction&gt; bk:status "pp. Boiler".
    </skos:example>
    <skos:example>
      &lt;bk:Transaction&gt; bk:status "in full Boiler".
    </skos:example>
    <skos:example>
      &lt;bk:Transaction&gt; bk:status "settled".
    </skos:example>
  </rdf:Property>
</rdf:RDF>
